Veir/Dialects/LLZK/Bool/OpInfo.lean
@@ -1,0 +1,97 @@
+module
+
+public import Veir.IR.Simp
+public import Veir.IR.OpInfo
+public import Veir.Verifier.Basic
+public import Veir.Dialects.LLZK.Bool.Properties
+meta import Veir.Meta.OpCode
+
+namespace Veir
+
+public section
+
+namespace LLZK
+
+@[opcodes]
+inductive Bool where
+| and
+| or
+| xor
+| not
+| assert
+| cmp
+deriving Inhabited, Repr, Hashable, DecidableEq
+
+end LLZK
+
+@[expose, properties_of]
+def LLZK.Bool.propertiesOf (op : LLZK.Bool) : Type :=
+match op with
+| .assert => BoolAssertProperties
+| .cmp => BoolCmpProperties
+| _ => Unit
+
+def LLZK.Bool.fromAttrDict
+    (op : LLZK.Bool) (attrDict : Std.HashMap ByteArray Attribute) :
+    Except String (LLZK.Bool.propertiesOf op) :=
+  match op with
+  | .and => .ok ()
+  | .or => .ok ()
+  | .xor => .ok ()
+  | .not => .ok ()
+  | .assert => BoolAssertProperties.fromAttrDict attrDict
+  | .cmp => BoolCmpProperties.fromAttrDict attrDict
+
+def LLZK.Bool.toAttrDict
+    (op : LLZK.Bool) (props : LLZK.Bool.propertiesOf op) :
+    Std.HashMap ByteArray Attribute :=
+  match op with
+  | .assert =>
+    match props.msg with
+    | some msg =>
+      (Std.HashMap.emptyWithCapacity 1).insert
+        "msg".toUTF8 (Attribute.stringAttr msg)
+    | none => Std.HashMap.emptyWithCapacity 0
+  | .cmp =>
+    (Std.HashMap.emptyWithCapacity 1).insert
+      "predicate".toUTF8 props.predicateAttr
+  | _ => Std.HashMap.emptyWithCapacity 0
+
+@[get_effects]
+def LLZK.Bool.getEffects
+    (op : LLZK.Bool) (_props : LLZK.Bool.propertiesOf op) : MemoryEffects :=
+  match op with
+  | .assert => .write
+  | .and | .or | .xor | .not | .cmp => .none
+
+def LLZK.Bool.isConstantLike (_op : LLZK.Bool) := false
+
+def LLZK.Bool.hasSSADominance (_op : LLZK.Bool) (_index : Nat) := true
+
+#generate_dialect LLZK.Bool
+
+instance : IsOpCode LLZK.Bool where
+  fromName := LLZK.Bool.fromName
+  name := LLZK.Bool.name
+  propertiesOf := LLZK.Bool.propertiesOf
+  fromAttrDict := LLZK.Bool.fromAttrDict
+  toAttrDict := LLZK.Bool.toAttrDict
+
+def LLZK.Bool.verifyLocalInvariants {OpInfo : Type} [IsOpCode OpInfo]
+    [HasDialect OpInfo LLZK.Bool] (opType : LLZK.Bool) (op : OperationPtr)
+    (ctx : WfIRContext OpInfo) (opIn : op.InBounds ctx.raw) : Except String PUnit := do
+  match opType with
+  | .and | .or | .xor => op.verifyPlainOpCounts ctx opIn 2 1
+  | .not => op.verifyPlainOpCounts ctx opIn 1 1
+  | .assert => op.verifyPlainOpCounts ctx opIn 1 0
+  | .cmp => op.verifyPlainOpCounts ctx opIn 2 1
+
+instance : HasOpInfo LLZK.Bool where
+  verifyLocalInvariants := LLZK.Bool.verifyLocalInvariants
+  getEffects := LLZK.Bool.getEffects
+  isConstantLike := LLZK.Bool.isConstantLike
+  hasSSADominance := LLZK.Bool.hasSSADominance
+
+end
+
+end Veir
