Veir/Dialects/LLZK/Cast/OpInfo.lean
@@ -1,0 +1,63 @@
+module
+
+public import Veir.IR.Simp
+public import Veir.IR.OpInfo
+public import Veir.Verifier.Basic
+meta import Veir.Meta.OpCode
+
+namespace Veir
+
+public section
+
+namespace LLZK
+
+@[opcodes]
+inductive Cast where
+| tofelt
+| toindex
+deriving Inhabited, Repr, Hashable, DecidableEq
+
+end LLZK
+
+@[expose, properties_of]
+def LLZK.Cast.propertiesOf (_op : LLZK.Cast) : Type := Unit
+
+def LLZK.Cast.fromAttrDict
+    (_op : LLZK.Cast) (_attrDict : Std.HashMap ByteArray Attribute) :
+    Except String (LLZK.Cast.propertiesOf _op) := .ok ()
+
+def LLZK.Cast.toAttrDict
+    (_op : LLZK.Cast) (_props : LLZK.Cast.propertiesOf _op) : Std.HashMap ByteArray Attribute :=
+  Std.HashMap.emptyWithCapacity 0
+
+def LLZK.Cast.getEffects (_op : LLZK.Cast) (_props : LLZK.Cast.propertiesOf _op) : MemoryEffects :=
+  .none
+
+def LLZK.Cast.isConstantLike (_op : LLZK.Cast) : Bool := false
+
+def LLZK.Cast.hasSSADominance (_op : LLZK.Cast) (_index : Nat) : Bool := true
+
+#generate_dialect LLZK.Cast
+
+instance : IsOpCode LLZK.Cast where
+  fromName := LLZK.Cast.fromName
+  name := LLZK.Cast.name
+  propertiesOf := LLZK.Cast.propertiesOf
+  fromAttrDict := LLZK.Cast.fromAttrDict
+  toAttrDict := LLZK.Cast.toAttrDict
+
+def LLZK.Cast.verifyLocalInvariants {OpInfo : Type} [IsOpCode OpInfo]
+    [HasDialect OpInfo LLZK.Cast] (opType : LLZK.Cast) (op : OperationPtr)
+    (ctx : WfIRContext OpInfo) (opIn : op.InBounds ctx.raw) : Except String PUnit := do
+  match opType with
+  | .tofelt | .toindex => op.verifyPlainOpCounts ctx opIn 1 1
+
+instance : HasOpInfo LLZK.Cast where
+  verifyLocalInvariants := LLZK.Cast.verifyLocalInvariants
+  getEffects := LLZK.Cast.getEffects
+  isConstantLike := LLZK.Cast.isConstantLike
+  hasSSADominance := LLZK.Cast.hasSSADominance
+
+end
+
+end Veir
